# baseURI: https://w3id.org/dprod//
# imports: http://purl.org/dc/terms/
# imports: http://www.w3.org/2004/02/skos/core
# imports: http://www.w3.org/ns/prov-o#
# imports: http://www.w3.org/ns/dcat
# prefix: dprod

@prefix dprod: <https://w3id.org/dprod/> .
@prefix dcat: <http://www.w3.org/ns/dcat#> .
@prefix dct: <http://purl.org/dc/terms/> .
@prefix dctype: <http://purl.org/dc/dcmitype/> .
@prefix foaf: <http://xmlns.com/foaf/0.1/> .
@prefix owl: <http://www.w3.org/2002/07/owl#> .
@prefix prov: <http://www.w3.org/ns/prov#> .
@prefix rdf: <http://www.w3.org/1999/02/22-rdf-syntax-ns#> .
@prefix rdfs: <http://www.w3.org/2000/01/rdf-schema#> .
@prefix sdo: <http://schema.org/> .
@prefix skos: <http://www.w3.org/2004/02/skos/core#> .
@prefix vcard: <http://www.w3.org/2006/vcard/ns#> .
@prefix xsd: <http://www.w3.org/2001/XMLSchema#> .
@prefix sh: <http://www.w3.org/ns/shacl#> .
@prefix dc: <ttp://purl.org/dc/elements/1.1/>.

<https://w3id.org/dprod/>
  a owl:Ontology ;
  dct:contributor [
      a foaf:Person ;
      sdo:affiliation [
          foaf:homepage <https://eccenca.com> ;
          foaf:name "eccenca GmbH" ;
        ] ;
      foaf:name "Marcel Fr√∂hlich" ;
    ] ;
  dct:contributor [
      a foaf:Person ;
      sdo:affiliation [
          foaf:homepage <https://ubs.com> ;
          foaf:name "UBS AG" ;
        ] ;
      foaf:name "Natasa Varytimou" ;
    ] ;
  dct:contributor [
      sdo:affiliation [
          foaf:homepage <https://brox.de> ;
          foaf:name "Brox IT-Solutions GmbH"
      ] ;
      foaf:name "Matthias Jurisch" ;
    ] ;
  dct:license <https://creativecommons.org/licenses/by/4.0/> ;
  dct:modified "2023-07-07"^^xsd:date ;
  rdfs:comment "DPROD is an RDF vocabulary designed to facilitate interoperability between data product descriptors."@en ;
  rdfs:label "The data product vocabulary"@en ;
  owl:imports dct: ;
  owl:imports <http://www.w3.org/2004/02/skos/core> ;
  owl:imports <http://www.w3.org/ns/prov-o#> ;
  owl:imports <http://www.w3.org/ns/dcat#> ;
  owl:versionInfo "Initial version of the dprod vocabulary. 07-07-2023 A Data Product has an owner and input, output datasets"@en ;
  foaf:maker [
      foaf:homepage <http://www.ekgf.org/> ;
      foaf:name "Enterprise Knowledge Graph Foundation" ;
    ] ;
.

dprod:DataProduct
  a rdfs:Class ;
  a owl:Class ;
  a sh:NodeShape ;
  rdfs:comment "A description of a data product as defined by the data mesh method"@en ;
  rdfs:isDefinedBy <https://w3id.org/dprod/> ;
  rdfs:label "Data Product"@en ;
  rdfs:subClassOf dcat:Resource ;
  skos:definition "A collection of metadata about a data product (e.g., ports and components.)"@en ;
  skos:scopeNote "A data product is typically represented as a single instance of this class."@en ;
  sh:property dprod:DataProduct-dataProductOwner;
  sh:property dprod:DataProduct-input;
  sh:property dprod:DataProduct-output;
.

dprod:DataProduct-dataProductOwner
  a sh:PropertyShape;
  rdfs:isDefinedBy <https://w3id.org/dprod>;
  sh:path dprod:dataProductOwner;
  sh:class dct:Agent;
  skos:definition "The Agent that is overall accountable for the data product. This includes managing the data product along its lifecycle ( creation, usage, versioning, deletion). "@en ;
  rdfs:label "DataProduct-dataProductOwner";
.

dprod:DataProduct-input
  a sh:PropertyShape;
  rdfs:isDefinedBy <https://w3id.org/dprod>;
  sh:path dprod:input;
  sh:class dcat:Dataset;
  skos:definition  "The dataset(s) that are included in the Data Product and can be the input of transformation efforts or surface in the product as is"@en ;
  rdfs:label "DataProduct-input;
.

dprod:DataProduct-output
  a sh:PropertyShape;
  rdfs:isDefinedBy <https://w3id.org/dprod>;
  sh:path dprod:output
  sh:class dcat:Dataset;
  skos:definition  "The dataset(s) that are created from the data product and become available in one or more distribution formats"@en ;
  rdfs:label "DataProduct-input;
.

dprod:Port
  a rdfs:Class ;
  a owl:Class ;
  rdfs:comment "A description of a port (e.g., input port, output port) of a data product"@en ;
  rdfs:isDefinedBy <https://w3id.org/dprod/> ;
  rdfs:label "Port"@en ;
  rdfs:subClassOf dcat:DataService ;
  skos:definition "A collection of metadata about a port (e.g., input port or output port.)"@en ;
.

dprod:fullyQualifiedName
  a rdf:Property ;
  a owl:DatatypeProperty ;
  rdfs:domain dcat:Resource ;
  rdfs:isDefinedBy <https://w3id.org/dprod/> ;
  rdfs:label "fully qualified name"@en ;
  rdfs:range xsd:string ;
  rdfs:comment "The fully qualified name of a resource."@en ;
.

dprod:domain
  a rdf:Property ;
  a owl:DatatypeProperty ;
  rdfs:domain dcat:Resource ;
  rdfs:isDefinedBy <https://w3id.org/dprod/> ;
  rdfs:label "domain"@en ;
  rdfs:range xsd:string ;
  rdfs:comment "The domain to which the data product belongs to."@en ;
.

dprod:outputPort
  a rdf:Property ;
  a owl:ObjectProperty ;
  rdfs:domain dprod:DataProduct ;
  rdfs:isDefinedBy <https://w3id.org/dprod/> ;
  rdfs:label "output port"@en ;
  rdfs:range dprod:Port ;
  rdfs:comment "An output port or a data product"@en ;
.

dprod:promise
  a rdf:Property ;
  a owl:ObjectProperty ;
  rdfs:domain dprod:Port ;
  rdfs:isDefinedBy <https://w3id.org/dprod/> ;
  rdfs:label "promise"@en ;
  rdfs:comment "A promise of a port"@en ;
.

dprod:expectation
  a rdf:Property ;
  a owl:ObjectProperty ;
  rdfs:domain dprod:Port ;
  rdfs:isDefinedBy <https://w3id.org/dprod/> ;
  rdfs:label "expectation"@en ;
  rdfs:comment "An expectation for a port"@en ;
.

dprod:contract
  a rdf:Property ;
  a owl:ObjectProperty ;
  rdfs:domain dprod:Port ;
  rdfs:isDefinedBy <https://w3id.org/dprod/> ;
  rdfs:label "contract"@en ;
  rdfs:comment "A contract for a port"@en ;
.

dprod:dataProductOwner
    a rdfs:ObjectProperty ;
    skos:definition "The Agent that is overall accountable for the data product. This includes managing the data product along its lifecycle ( creation, usage, versioning, deletion).. This can be different from the creator or the publisher of the Data Product "@en ;
    rdfs:isDefinedBy <https://w3id.org/dprod>;
    rdfs:label "data Product Owner";
    rdfs:domain dprod:DataProduct;
    rdfs:range dct:Agent;
    .

dprod:input
    a rdfs:ObjectProperty ;
    rdfs:label "input";
    skos:definition "The dataset(s) that are included in the Data Product and can be the input of transformation efforts or surface in the product as is"@en ;
    rdfs:isDefinedBy <https://w3id.org/dprod>;
    rdfs:domain dprod:DataProduct;
    rdfs:range dcat:Dataset;
    .

dprod:output
    a rdfs:ObjectProperty ;
    rdfs:label "output" ;
    skos:definition  "This is a generic property. In this case, it describes he dataset(s) that are created from the data product and become available in one or more distribution formats""@en ;
    rdfs:isDefinedBy <https://w3id.org/dprod>;
    rdfs:domain dprod:DataProduct;
    rdfs:range dcat:Dataset;
    .

